got instantiate_field working, yay!

Spec_sh.v
@@ -3,6 +3,7 @@
 
 Require Import List.
 Import ListNotations.
+Require Import String.
 
 (* Require Export Coq.Logic.Eqdep. *)
 
@@ -10,12 +11,10 @@ Add LoadPath "." as Specware.
 Require Import Specware.Util.
 
 
-Section Spec.
+(* Define the type of fields in one place, so we can change it later *)
 
-Class FieldType (F : Set) : Set :=
-  field_dec : forall (fld1 fld2 : F), {fld1=fld2} + {fld1<>fld2}.
-
-Context `{F_dec : FieldType}.
+Definition Field : Set := string.
+Definition Field_dec : forall (f1 f2 : Field), {f1=f2} + {f1<>f2} := string_dec.
 
 
 (**
@@ -25,13 +24,13 @@ Context `{F_dec : FieldType}.
 (* A Model is an element of the record type denoted by a Sig *)
 Inductive Model : Type :=
 | Model_Nil : Model
-| Model_Cons (fld:F) A (a : A) (M:Model) : Model
+| Model_Cons (fld:Field) A (a : A) (M:Model) : Model
 .
 
 (* A Spec is a partial Model of a Sig; README: Specs are indexed with
    their fields so that the fields they contain are known: i.e., even
    an inconsistent Spec has a fixed list of fields *)
-Inductive Spec : forall {flds : list F}, Type :=
+Inductive Spec : forall {flds : list Field}, Type :=
 | Spec_Nil : Spec (flds:=nil)
 | Spec_ConsNone f A {flds} :
     (forall (a:A), Spec (flds:=flds)) -> Spec (flds:= f :: flds)
@@ -41,7 +40,7 @@ Inductive Spec : forall {flds : list F}, Type :=
 .
 
 (* helper function for printing purposes *)
-Definition get_fields {flds} (spec : @Spec flds) := flds.
+Definition get_fields {flds} (spec : Spec (flds:=flds)) := flds.
 
 
 (**
@@ -51,7 +50,7 @@ Definition get_fields {flds} (spec : @Spec flds) := flds.
 (* Proof that field f is associated with type A in spec *)
 (* FIXME: the types (and elements!) depend on earlier elements! *)
 (*
-Inductive SpecElem (f : F) :
+Inductive SpecElem (f : Field) :
   forall A, option A -> forall {flds}, Spec (flds:=flds) -> Prop :=
 | SpecElem_BaseNone flds (spec : A -> Spec (flds:=flds)) :
     SpecElem f A None (Spec_ConsNone f A spec)
@@ -67,14 +66,14 @@ Inductive SpecElem (f : F) :
 *)
 
 (* Get the fields of a Model *)
-Fixpoint modelFields (M : Model) : list F :=
+Fixpoint modelFields (M : Model) : list Field :=
   match M with
     | Model_Nil => []
     | Model_Cons fld _ _ M' => fld :: modelFields M'
   end.
 
 (* Proof that field f is associated with element a of type A in model *)
-Inductive ModelElem (fld : F) A (a:A) : Model -> Prop :=
+Inductive ModelElem (fld : Field) A (a:A) : Model -> Prop :=
 | ModelElem_Base (model : Model) :
     ModelElem fld A a (Model_Cons fld A a model)
 | ModelElem_Cons fld' A' a' (model : Model) :
@@ -83,7 +82,7 @@ Inductive ModelElem (fld : F) A (a:A) : Model -> Prop :=
 .
 
 (* Model_Nil has no ModelElems *)
-Lemma not_ModelElem_nil (fld : F) A (a:A) :
+Lemma not_ModelElem_nil (fld : Field) A (a:A) :
   ModelElem fld A a Model_Nil -> False.
   assert (forall model,
             ModelElem fld A a model -> model = Model_Nil -> False).
@@ -101,7 +100,7 @@ Fixpoint modelProj (model : Model) :
     | Model_Nil => fun f in_nil => False_rect _ in_nil
     | Model_Cons f' A a _ model =>
       fun f in_pf =>
-        match F_dec f' f with
+        match Field_dec f' f with
             | left _ => existT id A a
             | right neq =>
               modelProj model f (or_proj_r _ _ neq in_pf)
@@ -116,7 +115,7 @@ Lemma modelProj_correct flds (model : Model (flds:=flds)) f in_pf :
   revert f in_pf; induction model; intros.
   elimtype False; apply in_pf.
   unfold modelProj; fold (modelProj (flds:=flds)).
-  destruct (F_dec f f0).
+  destruct (Field_dec f f0).
   rewrite <- e; apply ModelElem_Base.
   apply ModelElem_Cons.
   apply IHmodel.
@@ -230,22 +229,22 @@ Qed.
  **)
 
 (* A FieldMap is represented as a list of pairs *)
-Definition FieldMap := list (F * F).
+Definition FieldMap := list (Field * Field).
 
 (* The identity FieldMap *)
 Definition idFM : FieldMap := [].
 
 (* Apply a FieldMap to a F *)
-Fixpoint applyFM (m : FieldMap) (str : F) : F :=
+Fixpoint applyFM (m : FieldMap) (str : Field) : Field :=
   match m with
     | [] => str
     | (str_from, str_to) :: m' =>
-      if F_dec str str_from then str_to else
+      if Field_dec str str_from then str_to else
         applyFM m' str
   end.
 
 (* Applying idFM is the identity *)
-Lemma idFM_is_id (str : F) : applyFM idFM str = str.
+Lemma idFM_is_id (str : Field) : applyFM idFM str = str.
   reflexivity.
 Qed.
 
@@ -264,18 +263,18 @@ Lemma FieldMap_compose m1 m2 str :
   reflexivity.
   destruct a as [ str_from str_to ]; unfold composeFM; fold composeFM.
   unfold applyFM; fold applyFM.
-  destruct (F_dec str str_from).
+  destruct (Field_dec str str_from).
   reflexivity.
   apply IHm1.
 Qed.
 
 (* Return the list of Fs that map to an output F *)
-Fixpoint semiInvertFM (m : FieldMap) str : list F :=
+Fixpoint semiInvertFM (m : FieldMap) str : list Field :=
   match m with
     | [] => [str]
     | (str_from, str_to) :: m' =>
-      if F_dec str str_to then str_from :: semiInvertFM m' str
-      else remove F_dec str_from (semiInvertFM m' str)
+      if Field_dec str str_to then str_from :: semiInvertFM m' str
+      else remove Field_dec str_from (semiInvertFM m' str)
   end.
 
 (* semiInvertFM returns only Fs that map back to str *)
@@ -286,8 +285,8 @@ Lemma semiInvertFM_sound m str str' :
     [ rewrite H; reflexivity | destruct H ].
   destruct a as [ str_from str_to ]; unfold applyFM; fold applyFM.
   unfold semiInvertFM; fold semiInvertFM.
-  destruct (F_dec str str_to); intro in_pf;
-  destruct (F_dec str' str_from).
+  destruct (Field_dec str str_to); intro in_pf;
+  destruct (Field_dec str' str_from).
   rewrite e; reflexivity.
   apply IHm; destruct in_pf;
   [ elimtype False; apply n; rewrite H; reflexivity | assumption ].
@@ -301,9 +300,9 @@ Lemma semiInvertFM_complete m str str' :
   induction m; unfold applyFM; fold applyFM.
   intro e; left; symmetry; assumption.
   destruct a as [ str_from str_to ]; unfold semiInvertFM; fold semiInvertFM.
-  destruct (F_dec str' str_from); intro eApp.
+  destruct (Field_dec str' str_from); intro eApp.
   rewrite eApp; rewrite F_dec_true; left; symmetry; assumption.
-  destruct (F_dec str str_to).
+  destruct (Field_dec str str_to).
   right; apply IHm; assumption.
   apply remove_not_eq; [ assumption | apply IHm; assumption ].
 Qed.
@@ -352,7 +351,7 @@ Lemma spec_map_id {flds} (spec : Spec (flds:=flds)) :
                     (map id flds) flds (fun a => spec_map idFM (s a)) s
                     _ (fun fs => f :: fs)
                     _ (fun _ spec => Spec_ConsNone f A spec)).
-  apply (eq_dep_flds_fun _ F_dec); [ apply map_id | assumption ].
+  apply (eq_dep_flds_fun _ Field_dec); [ apply map_id | assumption ].
   apply (eq_dep_ctx _ (@Spec)
                     _ _ _ _ _ (fun fs => f :: fs) _ (fun _ => Spec_ConsSome f A a)
                     IHspec).
@@ -415,7 +414,7 @@ Lemma spec_map_comp {flds} (spec : Spec (flds:=flds)) m1 m2 :
                     _ (fun fs => applyFM m2 (applyFM m1 f) :: fs)
                     _ (fun _ spec => Spec_ConsNone (applyFM m2 (applyFM m1 f)) A spec)
         ).
-  apply (eq_dep_flds_fun _ F_dec);
+  apply (eq_dep_flds_fun _ Field_dec);
     [ rewrite map_map; apply map_ext;
       intro fld; symmetry; apply FieldMap_compose
     | assumption ].
@@ -500,13 +499,13 @@ Qed.
  **)
 
 (* Apply Model_Cons once for each field name in a list *)
-Fixpoint multi_Model_Cons (flds : list F) A (a : A) model :=
+Fixpoint multi_Model_Cons (flds : list Field) A (a : A) model :=
   match flds with
     | [] => model
     | fld :: flds' => Model_Cons fld A a (multi_Model_Cons flds' A a model)
   end.
 
-Lemma In_multi_Model_Cons (flds : list F) A (a : A) model f :
+Lemma In_multi_Model_Cons (flds : list Field) A (a : A) model f :
   In f flds -> ModelElem f A a (multi_Model_Cons flds A a model).
   induction flds; intro in_pf.
   inversion in_pf.
@@ -515,7 +514,7 @@ Lemma In_multi_Model_Cons (flds : list F) A (a : A) model f :
   apply ModelElem_Cons; apply IHflds; assumption.
 Qed.
 
-Lemma multi_Model_Cons_ModelElem (flds : list F) A (a : A) model f A' a' :
+Lemma multi_Model_Cons_ModelElem (flds : list Field) A (a : A) model f A' a' :
   ModelElem f A' a' model ->
   ModelElem f A' a' (multi_Model_Cons flds A a model).
   induction flds; intro melem.
@@ -523,7 +522,7 @@ Lemma multi_Model_Cons_ModelElem (flds : list F) A (a : A) model f A' a' :
   apply ModelElem_Cons; apply IHflds; assumption.
 Qed.
 
-Lemma multi_Model_Cons_un_ModelElem (flds : list F) A (a : A) model f A' a' :
+Lemma multi_Model_Cons_un_ModelElem (flds : list Field) A (a : A) model f A' a' :
   ModelElem f A' a' (multi_Model_Cons flds A a model) ->
   (In f flds /\ eq_dep _ id A a A' a') \/ ModelElem f A' a' model.
   revert A a model f A' a'; induction flds; intros.
@@ -676,7 +675,7 @@ Lemma IsMorphism_map {flds1} (spec1 : Spec (flds:=flds1))
   IDEA: "un-map" a model along an m, given a set of input fields:
   - un-mapping should depend only on m and flds
   - NOTE: might duplicate some fields, since model might have duplicate fields,
-    so we define unmap_flds : flds -> m -> model -> list F and
+    so we define unmap_flds : flds -> m -> model -> list Field and
     unmap : forall flds m model, Model (flds:=unmap_flds flds m model)
   - need IsModel model (spec_map m spec) <-> IsModel (unmap flds m model) spec
   - can then unmap, pass to the original IsMorphism, and then undo the unmapping
@@ -708,8 +707,6 @@ Definition mcompose {flds1} {spec1 : Spec (flds:=flds1)}
   mkMorphism spec1 spec3 (composeFM (projMorph morph1) (projMorph morph2))
              (IsMorphism_trans _ _ _ _ _ (projMorph_pf morph1) (projMorph_pf morph2)).
 
-
-End Spec.
 
 (**
  ** Syntax for specs and morphism
