Refinement_sh.v
@@ -1,0 +1,443 @@
+
+(*** Tactics for Refinement ***)
+
+Require Import String.
+
+Add LoadPath "." as Specware.
+Require Import Specware.Util.
+Require Export Specware.Spec_sh.
+
+Import ListNotations.
+Require Export Coq.Logic.Eqdep.
+
+
+(*** Refinements and helper defs ***)
+
+(* a Refinement of a spec is another spec and a morphism to it *)
+Inductive Refinement {flds} (spec : Spec (flds:=flds)) : Type :=
+| mkRefinement {flds'} (spec' : Spec (flds:=flds')) (morph : Morphism spec spec')
+  : Refinement spec.
+
+(* An existential type for a spec that hides the fields when printing *)
+Inductive SomeSpec : Type :=
+| mkSomeSpec {flds : list Field} (spec : Spec (flds:=flds)) : SomeSpec.
+
+(* Extracting the destination spec of a Refinement *)
+Definition refinementSpec {flds} {spec : Spec (flds:=flds)} (ref : Refinement spec) : SomeSpec :=
+  match ref with
+    | mkRefinement _ spec' _ => mkSomeSpec spec'
+  end.
+
+(*** The simplest refinement tactic: finish refinement (you're done) ***)
+
+(* The identity refinement *)
+Definition id_refinement {flds} spec : Refinement (flds:=flds) spec :=
+  mkRefinement spec spec (mid _).
+
+(* the tactic the ends refinement, giving the current spec being refined as the output *)
+Ltac end_refine := apply id_refinement.
+
+
+(*** A Refinement step that applies a morphism ***)
+
+(* Applying a morphism to prove a refinement goal *)
+Definition apply_morphism_fun {flds1} {spec1 : Spec (flds:=flds1)}
+           {flds2} {spec2 : Spec (flds:=flds2)}
+           (m12 : Morphism spec1 spec2) :
+  Refinement spec2 ->
+  Refinement spec1.
+  intro ref2; destruct ref2 as [ flds3 spec3 m23 ].
+  apply (mkRefinement _ spec3);
+  apply (mcompose m12 m23).
+Defined.
+
+(* The above as a tactic, so we don't have to write "apply apply_morphism" *)
+Ltac apply_morphism morph := apply (apply_morphism_fun morph).
+
+
+(*** Refinement of sub-specs ***)
+
+Definition IsMorphism_ConsNone f A {flds1} spec1 {flds2} spec2 m :
+  (forall a, IsMorphism (flds1:=flds1) (spec1 a) (flds2:=flds2) (spec2 a) m) ->
+  IsMorphism (Spec_ConsNone f A spec1) (Spec_ConsNone (applyFM m f) A spec2) m.
+  intros ismorph model ism.
+  destruct ism as [ a sig ]; destruct sig as [ melem ism ].
+  exists a; split; [ | apply ismorph ]; assumption.
+Qed.
+
+Definition IsMorphism_ConsSome f A a {flds1} spec1 {flds2} spec2 m :
+  IsMorphism (flds1:=flds1) spec1 (flds2:=flds2) spec2 m ->
+  IsMorphism (Spec_ConsSome f A a spec1) (Spec_ConsSome (applyFM m f) A a spec2) m.
+  intros ismorph model ism.
+  destruct ism as [ melem ism ]; split; [ | apply ismorph ]; assumption.
+Qed.
+
+
+(*** Instantiating a field in a spec ***)
+
+(* a refinement using the idFM FieldMap *)
+Inductive IdRefinement {flds} (spec : Spec (flds:=flds)) : Type :=
+| mkIdRefinement (spec' : Spec (flds:=flds)) (ism : IsMorphism spec spec' idFM)
+  : IdRefinement spec.
+
+Definition IdRefinement_projSpec {flds} {spec} (idr : @IdRefinement flds spec) :
+  Spec (flds:=flds) :=
+  match idr with
+    | mkIdRefinement spec' _ => spec'
+  end.
+
+Definition IdRefinement_projIsM {flds} {spec} (idr : @IdRefinement flds spec) :
+  IsMorphism spec (IdRefinement_projSpec idr) idFM :=
+  match idr with
+    | mkIdRefinement spec' ism => ism
+  end.
+
+(* proof that instantiating the first element of a spec yields a morphism *)
+Lemma IsMorphism_instantiate_base f A a {flds} (spec : A -> Spec (flds:=flds)) :
+  IsMorphism (Spec_ConsNone f A spec) (Spec_ConsSome f A a (spec a)) idFM.
+  intros model ism; destruct ism.
+  exists a; split;
+  [ rewrite idFM_is_id | rewrite spec_map_id ]; assumption.
+Qed.
+
+(* instantiate the first element of a spec *)
+Definition instantiate_field_base f {A} (a:A) {flds} (spec : A -> Spec (flds:=flds)) :
+  IdRefinement (Spec_ConsNone f A spec) :=
+  mkIdRefinement _ (Spec_ConsSome f A a (spec a))
+                 (IsMorphism_instantiate_base _ _ _ _).
+
+(*
+Definition instantiate_field_base f {A} (a:A) {flds} (spec : A -> Spec (flds:=flds)) :
+  { spec' : Spec (flds:=f :: flds) | IsMorphism (Spec_ConsNone f A spec) spec' idFM } :=
+  existT _ (Spec_ConsSome f A a (spec a)) (IsMorphism_instantiate_base _ _ _ _).
+*)
+
+(* skip the first element of a ConsNone spec and instantiate the rest *)
+Definition instantiate_field_None f A {flds} {spec : A -> Spec (flds:=flds)}
+           (fn : forall a, IdRefinement (spec a)) :
+  IdRefinement (Spec_ConsNone f A spec) :=
+  mkIdRefinement _ (Spec_ConsNone f A (fun a => IdRefinement_projSpec (fn a)))
+         (IsMorphism_ConsNone
+            f A spec _ idFM
+            (fun a => IdRefinement_projIsM (fn a))).
+
+(*
+Definition instantiate_field_None f A {flds} {spec : A -> Spec (flds:=flds)}
+  (fn : forall a, { spec' : Spec (flds:=flds) |
+                    IsMorphism (spec a) spec' idFM }) :
+  { spec' : Spec (flds:=f :: flds) | IsMorphism (Spec_ConsNone f A spec) spec' idFM } :=
+  existT _ (Spec_ConsNone f A (fun a => projT1 (fn a)))
+         (IsMorphism_ConsNone
+            f A spec _ idFM
+            (fun a => projT2 (fn a))).
+*)
+
+(* skip the first element of a ConsSome spec and instantiate the rest *)
+Definition instantiate_field_Some f A a {flds} {spec : Spec (flds:=flds)}
+  (rest : IdRefinement spec) :
+  IdRefinement (Spec_ConsSome f A a spec) :=
+  mkIdRefinement _ (Spec_ConsSome f A a (IdRefinement_projSpec rest))
+                 (IsMorphism_ConsSome f A a spec _ _ (IdRefinement_projIsM rest)).
+
+(*
+Definition instantiate_field_Some f A a {flds} {spec : Spec (flds:=flds)}
+  (rest : { spec' : Spec (flds:=flds) | IsMorphism spec spec' idFM }) :
+  { spec' : Spec (flds:=f :: flds) | IsMorphism (Spec_ConsSome f A a spec) spec' idFM } :=
+  existT _ (Spec_ConsSome f A a (projT1 rest))
+         (IsMorphism_ConsSome f A a spec _ _ (projT2 rest)).
+*)
+
+Definition test_spec_fun :=
+  Spec_ConsNone "T"%string Set (fun T =>
+  Spec_ConsNone "f"%string (T -> T) (fun f =>
+  Spec_Nil)).
+
+Definition test_spec_fun2 : Refinement test_spec_fun.
+  assert (IdRefinement test_spec_fun) as H; [ | end_refine ].
+  unfold test_spec_fun.
+  apply instantiate_field_None; intro T.
+  apply (instantiate_field_base "f"%string ((fun X (x:X) => x) T)).
+Qed.
+
+(* A helper tactic which repeatedly tries to apply instantiate_field_* above *)
+Ltac instantiate_helper f fs val :=
+  compute;
+  lazymatch goal with
+    | |- (IdRefinement (Spec_ConsNone f ?A ?rest)) =>
+      lazymatch (eval compute in fs) with
+        | nil => apply (instantiate_field_base f val)
+        | _ => fail "Could not apply all supplied fields!"
+      end
+    | |- (IdRefinement (Spec_ConsNone ?f_cur ?A ?rest)) =>
+      lazymatch (eval compute in fs) with
+        | (f_cur :: ?fs_rest) =>
+          let var := fresh "a" in
+          apply instantiate_field_None; intro var;
+          instantiate_helper f fs_rest (val var)
+        | _ =>
+          let var := fresh "a" in
+          apply instantiate_field_None; intro var;
+          instantiate_helper f fs val
+      end
+    | |- (IdRefinement (Spec_ConsSome ?f_cur ?A ?a ?rest)) =>
+      lazymatch (eval compute in fs) with
+        | (f_cur :: ?fs_rest) =>
+          apply instantiate_field_Some;
+          instantiate_helper f fs_rest (val a)
+        | _ =>
+          apply instantiate_field_Some;
+          instantiate_helper f fs val
+      end
+    | |- _ => fail "instantiate_helper: not an IdRefinement goal!"
+  end.
+(*
+  repeat (apply (instantiate_field_base f val) ||
+          apply instantiate_field_None ||
+          apply instantiate_field_Some).
+*)
+
+Ltac instantiate_helper_debug f fs val :=
+  compute;
+  lazymatch goal with
+    | |- (IdRefinement (Spec_ConsNone f ?A ?rest)) =>
+      lazymatch (eval compute in fs) with
+        | nil => apply (instantiate_field_base f val)
+        | _ => fail "Could not apply all supplied fields!"
+      end
+    | |- (IdRefinement (Spec_ConsNone ?f_cur ?A ?rest)) =>
+      lazymatch (eval compute in fs) with
+        | (f_cur :: ?fs_rest) =>
+          let var := fresh "a" in
+          apply instantiate_field_None; intro var;
+          instantiate_helper_debug f fs_rest (val var)
+        | _ =>
+          let var := fresh "a" in
+          apply instantiate_field_None; intro var;
+          instantiate_helper_debug f fs val
+      end
+    | |- (IdRefinement (Spec_ConsSome ?f_cur ?A ?a ?rest)) =>
+      lazymatch (eval compute in fs) with
+        | (f_cur :: ?fs_rest) =>
+          apply instantiate_field_Some;
+          instantiate_helper_debug f fs_rest (val a)
+        | _ =>
+          apply instantiate_field_Some;
+          instantiate_helper_debug f fs val
+      end
+    | |- _ => idtac "instantiate_helper_debug: not an IdRefinement goal!"
+  end.
+
+(* The tactic itself *)
+Ltac instantiate_field f fs val :=
+  lazymatch goal with
+    | |- Refinement ?spec =>
+      let H := fresh "H" in
+      let ism := fresh "isMorph" in
+      assert (IdRefinement spec) as H; [ instantiate_helper f fs val | ];
+      destruct H as [ spec' ism ];
+      apply_morphism (mkMorphism spec spec' idFM ism)
+    | _ => fail "Not a refinement goal!"
+  end.
+
+(* Debugging version, which does not call instantiate_helper *)
+Ltac instantiate_field_start :=
+  lazymatch goal with
+    | |- Refinement ?spec =>
+      let H := fresh "H" in
+      let ism := fresh "isMorph" in
+      assert (IdRefinement spec) as H; [ | end_refine ]
+    | _ => fail "Not a refinement goal!"
+  end.
+
+Ltac instantiate_field_debug f fs val :=
+  lazymatch goal with
+    | |- Refinement ?spec =>
+      let H := fresh "H" in
+      let ism := fresh "isMorph" in
+      assert (IdRefinement spec) as H;
+        [ instantiate_helper_debug f fs val | ]
+    | _ => fail "Not a refinement goal!"
+  end.
+
+Definition test_spec1 :=
+  Spec_ConsSome "T"%string Set nat (
+  Spec_ConsNone "f"%string (nat -> nat) (fun f =>
+  Spec_Nil)).
+
+(* Instance string_FieldType : FieldType string := string_dec. *)
+
+Definition test_spec2 : Refinement test_spec1.
+  instantiate_field "f"%string ([]:list string) (fun (x:nat) => x).
+  end_refine.
+Defined.
+
+Eval compute in (refinementSpec test_spec2).
+
+
+Definition test_spec3 :=
+  Spec_ConsNone "T"%string Set (fun T =>
+  Spec_ConsNone "f"%string (T -> T) (fun f =>
+  Spec_Nil)).
+
+(* Instance string_FieldType : FieldType string := string_dec. *)
+
+Definition test_spec4 : Refinement test_spec3.
+  instantiate_field "f"%string (["T"%string]) (fun T (x:T) => x).
+  end_refine.
+Defined.
+
+Eval compute in (refinementSpec test_spec4).
+
+
+  instantiate_helper_debug "f"%string fs (fun X (x:X) => x). *)
+  (* apply instantiate_field_None. *)
+  instantiate_field_start.
+  compute. apply instantiate_field_None.
+  let my_fs := (eval compute in fs) in
+  lazymatch goal with
+    | |- (IdRefinement (Spec_ConsNone ?f_cur ?A ?rest)) =>
+      lazymatch my_fs with
+        | (f_cur :: ?fs_rest) =>
+          let var := fresh "a" in
+          apply instantiate_field_None; intro var
+        | _ => fail "aaaaahhhhh2"
+      end
+  end.
+
+
+  end_refine.
+Defined.
+
+Eval compute in (refinementSpec test_spec4).
+
+
+  instantiate_field_debug.
+  compute -[IsMorphism].
+  lazymatch eval compute in test_spec1 with
+    | { spec' : @Spec ?flds
+         | IsMorphism (Spec_ConsSome ?f_cur ?A ?a ?rest) spec' idFM } =>
+      fail "aaaahhhh"
+  end.
+
+
+  instantiate_field "f"%string ([]:list string) (fun (x:nat) => x).
+  (*
+  unfold test_spec1.
+  lazymatch goal with
+    | |- { spec' : @Spec ?flds
+         | IsMorphism (Spec_ConsSome ?f_cur ?A ?a ?rest) spec' idFM } =>
+      fail "aaaahhhh"
+  end. *)
+  lazymatch goal with
+    | |- ?gl => let gl_eval := (eval compute in gl) in assert gl_eval
+  end.
+
+  let foo := eval compute in test_spec1 in assert (foo=foo).
+  lazymatch eval compute in test_spec1 with
+    | { spec' : @Spec ?flds
+         | IsMorphism (Spec_ConsSome ?f_cur ?A ?a ?rest) spec' idFM } =>
+      fail "aaaahhhh"
+  end.
+  instantiate_field "f"%string ([]:list string) (fun (x:nat) => x).
+  end_refine.
+Qed.
+
+Definition test_spec_fun :=
+  Spec_ConsNone "T" Set (fun T =>
+  Spec_ConsNone "f" (T -> T) (fun f =>
+  Spec_Nil)).
+
+(* Set Ltac Debug. *)
+
+Definition test_spec_id : Refinement test_spec_fun.
+  assert ({ spec' : @Spec ["T"%string; "f"%string ] | IsMorphism test_spec_fun spec' idFM }) as H.
+  instantiate_helper ("T"%string) (fun (x:nat) => x).
+
+  instantiate_field ("f"%string) (fun T (x:T) => x).
+
+Eval compute in (get_fields test_spec_fun).
+
+Definition test_spec_id : Refinement test_spec_fun.
+  assert ({ spec' : @Spec ["T"%string; "f"%string ] | IsMorphism test_spec_fun spec' idFM }) as H.
+  apply instantiate_field_None; intro a.
+  apply (instantiate_field_base (fun x => x)).
+  destruct H as [ spec' ismorph ]; apply_morphism (mkMorphism _ _ _ ismorph).
+  end_refine.
+Defined.
+
+Eval compute in (refinementSpec test_spec_id).
+
+
+
+Definition test_spec_id :=
+  Spec_ConsNone "T" Set (fun T =>
+  Spec_ConsSome "idT" (T -> T) (fun t => t)
+  Spec_Nil).
+
+Definition test_spec_id_nat :=
+  Spec_ConsSome "T" Set nat (
+  Spec_ConsSome "idT" (nat -> nat) (fun t => t)
+  Spec_Nil).
+
+(* FIXME: cannot get type-class resolution to work here... *)
+(*
+Section instantiation.
+
+  Class InstantiatesTo
+        {flds1} (spec1 : Spec (flds:=flds1))
+        {flds2} (spec2 : Spec (flds:=flds2)) : Prop :=
+    instantiation_ismorph_id : IsMorphism spec1 spec2 idFM.
+
+  Variables (flds:list string) (fld:string) (A:Type) (a:A)
+            (spec:A -> Spec (flds:=flds)).
+
+  Global Instance InstantiatesTo_Base :
+    InstantiatesTo (Spec_ConsNone fld A spec) (Spec_ConsSome fld A a (spec a)).
+  intros model ism; destruct ism.
+  exists a; split;
+  [ rewrite idFM_is_id | rewrite spec_map_id ]; assumption.
+  Qed.
+
+  (*
+  Definition test1 :
+    InstantiatesTo (Spec_ConsNone fld A spec) (Spec_ConsSome fld A a (spec a))
+    := instantiation_ismorph_id.
+   *)
+
+End instantiation.
+*)
+
+
+(*
+Program Definition instantiate_helper_step_ConsNone
+           f A {flds} (spec : A -> Spec (flds:=flds))
+           (F : forall a,
+                  { spec' : Spec (flds:=flds) & IsMorphism (spec a) spec' id }) :
+  { spec' : Spec (flds:= f :: flds)
+                 & IsMorphism (Spec_ConsNone f A spec) spec' id } :=
+  existT (fun spec' => IsMorphism _ spec' id)
+         ({# f ::: A ; a => projT1 (F a) #})
+         (fun model2 ism2 =>
+            existT2 (fun _ => _) (fun _ => _) model2
+                    _ _).
+Obligation 1.
+apply (IsModel_ConsNone)
+
+  apply (match )
+
+Definition instantiate_helper_step_ConsSome
+           f A a {flds} (spec : A -> Spec (flds:=flds)) :
+  { spec' : Spec (flds:= f :: flds) & IsMorphism (Spec_ConsNone f A spec) spec' id } :
+*)
+
+Ltac instantiate_field f val :=
+  match goal with
+    | |- Refinement ?flds ?spec =>
+      let H := fresh "H" in
+      let spec' := fresh "spec" in
+      let ism := fresh "isMorph" in
+      assert ({ spec' : Spec (flds:=flds) | IsMorphism spec spec' id }) as H; [ instantiate_helper f val spec | ];
+      destruct H as [ spec' ism ];
+      apply (apply_morphism (mkMorphism spec spec' id ism))
+    | _ => fail "Not a refinement goal!"
+  end.
